$$T=\ln(\tau)$$

# Equivalent Forms ðŸ˜­ðŸ˜­ðŸ˜­ðŸ˜­ðŸ˜­ðŸ˜­ðŸ˜­ðŸ˜­ðŸ˜­ðŸ˜­

The mathematical formula $T = \ln(\tau)$ can be expressed in various equivalent forms, depending on the mathematical attributes or application contexts we want to emphasize. Here are some common equivalent forms:

## 1. Inverse Transformation
- To revert from $T$ back to $\tau$:

  $$\tau = e^T$$
  
  where $e$ is the base of the natural logarithm, approximately equal to 2.71828.

## 2. Exponential Form
- Rewrite $T$ in the exponential form of \(\tau\):
  
  $$e^T = \tau$$

## 3. Change of Logarithm Base
- If we want to use a different base $b$ (like 10), we can rewrite the formula as:
  
  $$T = \frac{\log_b(\tau)}{\log_b(e)}$$
  
  Because $\ln(\tau) = \log_e(\tau)$, $\log_b(e)$ is the factor necessary to convert the natural logarithm to a logarithm with base $b$.

## 4. Integral Form
- $T$ can be seen as the integral of $\frac{1}{\tau}$:
  
  $$T = \int_1^\tau \frac{1}{x} \, dx$$
  
  This is because $\ln(\tau)$ is the indefinite integral of $\frac{1}{x}$.

## 5. Complex Number Form
- In the domain of complex numbers, $T = \ln(\tau)$ can be extended to:
  
  $$T = \ln(|\tau|) + i \arg(\tau)$$
  
  where $i$ is the imaginary unit, $|\tau|$ is the modulus of $\tau$, and $\arg(\tau)$ is the argument of $\tau$.

## 6. Function and Its Inverse
- Considering $T$ as the inverse function of $\tau$:
  
  $$\tau = f^{-1}(T)$$
  
  where $f(T) = e^T$ is the inverse function of $T$.


$K = \frac{1}{\ln(b)}$
-----------------------
obtaining the logarithmic time scale and introducing He's scaling constant, starting from the assumption that the cosmological constant evolves as $\Lambda(t) = 1/t$:

**1. Re-Assumption of Cosmological Constant Evolution**

* We assume that the cosmological constant $\Lambda(t)$ evolves with linear time $t$ according to the following relationship:

    $$\Lambda(t) = \frac{1}{t}$$

**2. Definition of New Time Scale T**

* We define a new time scale $T$ by integrating the cosmological constant $\Lambda(t)$ with respect to $t$:

    $$T = \int \Lambda(t) \, dt = \int \frac{1}{t} \, dt$$

**3. Calculation of the Integral**

* Performing the above integration yields:

    $$T = \ln(t) + C$$
    where $C$ is an integration constant.

**4. Introduction of a New Time Parameter Ï„**

* We neglect the integration constant $C$ and introduce a new time parameter $\tau$, such that:

    $$\tau = t$$

*  Therefore, the new time scale $T$ can be expressed as:

    $$T = \ln(\tau)$$
  Here, we have obtained the desired logarithmic time scale.

**5. Introduction of a Different Logarithmic Base $b$ and He's Scaling Constant $\Lambda_b$**

* To consider different logarithmic bases, we define a new time scale $T_b$ using a base $b$:

    $$T_b = \log_b(\tau)$$

* Using the change of base formula for logarithms, we can relate $T_b$ to the natural logarithm:

    $$T_b = \frac{\ln(\tau)}{\ln(b)}$$

* We define He's scaling constant $\Lambda_b$ as:

    $$\Lambda_b = \ln(b)$$

* Substituting $\Lambda_b$, we obtain the relationship between $T_b$ and $T$:

    $$T_b = \frac{\ln(\tau)}{\ln(b)} = \frac{T}{\ln(b)} = \frac{T}{\Lambda_b}$$

**Conclusion**

Through the steps above, we have completed the process of deriving the logarithmic time scale $T = \ln(\tau)$ and introducing He's scaling constant $\Lambda_b$, starting from the assumption that the cosmological constant evolves as $\Lambda(t) = 1/t$.

1.  **Assumption:** We assume the cosmological constant $\Lambda(t)$ evolves with linear time $t$ such that $\Lambda(t) = 1/t$.
2.  **New Time Scale:** By integration, we define a new time scale $T = \ln(t)$.
3.  **New Time Parameter:** We set $\tau = t$, then $T = \ln(\tau)$.
4.  **He's Scaling Constant:** We introduce He's scaling constant $\Lambda_b = \ln(b)$ allowing us to relate different logarithmic time scales through: $T_b = \frac{T}{\Lambda_b}$.



